lean/Environments.lean
@@ -1,9 +1,14 @@
 import .Cyclone_Formal_Syntax
 
-/- This is the most general binds and ok that I can make, 
+/- 
+ This is the most general binds and ok that I can make, 
  involving an instance of a decidable type class that 
- Lean must find. None must have its full type in 
- some of these examples.
+ Lean must find. 
+ So I'll need typeclasses and instances to make this work.
+ Do I want this that general or as in the coq model with different specializations.
+ Not sure what lemmas and meta programming we'll need for ok and binds. 
+ Will have to see them in action in a theorem. 
+
 -/
 
 def binds {key : Type} [eq : decidable_eq key] {value : Type} : key → list (key × value) → option value
@@ -37,6 +42,42 @@ lemma binds_string_none {value : Type}:
 begin
   simp,
 end 
+
+/- Check which binds's can find a type instance, they all work with
+ a simple @[derive decidable_eq]
+
+lemma binds_Heap_some (v : Var) (h : Heap) (e : E) :
+   binds v h = some e := 
+sorrycharlie
+
+lemma binds_Heap_none (v : Var) (h : Heap):
+   binds v h = none := 
+sorrycharlie
+
+lemma binds_Delta_some (v : Var) (d : Delta) (k : Kappa) :
+   binds v d = some k := 
+sorrycharlie
+
+lemma binds_Delta_none (v : Var) (d : Delta) :
+   binds v d = none := 
+sorrycharlie
+
+lemma binds_Gamma_some (v : Var) (g : Gamma) (t : Tau) : 
+   binds v g = some t := 
+sorrycharlie
+
+lemma binds_Gamma_none (v : Var) (g : Gamma) : 
+   binds v g = none := 
+sorrycharlie
+
+lemma binds_Upsilon_some (v : Var) (p : Path) (u : Upsilon) (t : Tau) : 
+   binds (v,p) u = some t := 
+sorrycharlie
+
+lemma binds_Upsilon_none (v : Var) (p : Path) (u : Upsilon) : 
+   binds (v,p) u = none := 
+sorrycharlie
+-/
 
 /- Evals don't work as you can't print a prop. -/
 
@@ -75,7 +116,7 @@ begin
  induction' h,
 end
 
-/- To hard, let's get some more lemmas. -/ 
+/- Too hard, let's get some more lemmas. -/ 
 lemma ok₃ : ok [("fred",1),("joe",2)] :=
 begin
   apply ok.notin,
@@ -83,3 +124,27 @@ begin
   cc,
   simp,
 end
+
+
+/- Check which ok's can find a type instance, they all work with
+ a simple @[derive decidable_eq].
+-/
+-- lemma ok_Heap (h : Heap) :
+--    ok h := 
+-- sorrycharlie
+-- 
+-- lemma ok_Delta (d : Delta) :
+--   ok d :=
+-- sorrycharlie
+-- 
+-- lemma ok_Gamma (g : Gamma) :
+--  ok g  :=
+-- sorrycharlie 
+--
+-- lemma ok_Upsilon (u : Upsilon) :
+--  ok u :=
+-- sorrycharlie
+
+
+
+
